Clean/Air/Extraction/IR.lean
@@ -120,6 +120,8 @@ structure FixedColumnsProgram (F : Type) where
   rows : List (Array F)
 
 structure ComponentProgram (F : Type) [FiniteField F] where
+  name : String
+  dataColumns : List ℕ
   inputWidth : ℕ
   fixedColumns : Option (FixedColumnsProgram F)
   width : ℕ
